tuning

Weidenbach_Book/IsaSAT.thy
@@ -166,30 +166,10 @@ sepref_definition (in -) empty_init_code'
 declare empty_init_code'.refine[sepref_fr_rules]
 
 
-text \<open>
-  This is a trick to recover from consumption of a variable (\<^term>\<open>\<A>\<^sub>i\<^sub>n\<close>) that is passed as
-  argument and destroyed by the initialisation: We copy it as a zero-cost
-  (by creating a \<^term>\<open>()\<close>), because we don't need it in the code and only in the specification.
-
-  TODO rename to ghost
-\<close>
-definition virtual_copy where
-  [simp]: \<open>virtual_copy = id\<close>
-
-definition virtual_copy_rel where
-  \<open>virtual_copy_rel = {(c, b). c = ()}\<close>
-
-abbreviation virtual_copy_assn where
-  \<open>virtual_copy_assn \<equiv> hr_comp unit_assn virtual_copy_rel\<close>
-
-lemma [sepref_fr_rules]:
-  \<open>(return o (\<lambda>_. ()), RETURN o virtual_copy) \<in> R\<^sup>k \<rightarrow>\<^sub>a virtual_copy_assn\<close>
-  by sepref_to_hoare (sep_auto simp: virtual_copy_rel_def)
-
 lemma init_dt_wl_code_refine[sepref_fr_rules]:
   \<open>(uncurry2 (\<lambda>_. init_dt_wl_code), uncurry2 (isasat_input_ops.init_dt_wl_heur))
   \<in> [\<lambda>((N, S), S'). isasat_input_bounded \<A>\<^sub>i\<^sub>n \<and> N = \<A>\<^sub>i\<^sub>n]\<^sub>a
-    virtual_copy_assn\<^sup>k *\<^sub>a (list_assn (list_assn unat_lit_assn))\<^sup>d *\<^sub>a (isasat_input_ops.isasat_init_assn \<A>\<^sub>i\<^sub>n)\<^sup>d \<rightarrow>
+    ghost_assn\<^sup>k *\<^sub>a (list_assn (list_assn unat_lit_assn))\<^sup>d *\<^sub>a (isasat_input_ops.isasat_init_assn \<A>\<^sub>i\<^sub>n)\<^sup>d \<rightarrow>
     isasat_input_ops.isasat_init_assn \<A>\<^sub>i\<^sub>n\<close>
   unfolding PR_CONST_def
   unfolding hfref_def hn_refine_def
@@ -201,13 +181,13 @@ lemma init_dt_wl_code_refine[sepref_fr_rules]:
       rule_format, of \<open>(snd (fst c), snd c)\<close> \<open>(snd (fst a), snd a)\<close>]
     by (cases a)
        (sep_auto dest!: frame_rule_left[of \<open>_ * isasat_input_ops.isasat_init_assn _ _ _\<close> _ _
-            \<open>virtual_copy_assn \<A>\<^sub>i\<^sub>n (fst (fst a))\<close>])
+            \<open>ghost_assn \<A>\<^sub>i\<^sub>n (fst (fst a))\<close>])
   done
 (*
 lemma init_dt_wl_fast_code_refine[sepref_fr_rules]:
   \<open>(uncurry2 (\<lambda>_. init_dt_wl_fast_code), uncurry2 (isasat_input_ops.init_dt_wl_heur_fast))
   \<in> [\<lambda>((N, S), S'). isasat_input_bounded \<A>\<^sub>i\<^sub>n \<and> N = \<A>\<^sub>i\<^sub>n]\<^sub>a
-    virtual_copy_assn\<^sup>k *\<^sub>a (list_assn (list_assn unat_lit_assn))\<^sup>d *\<^sub>a
+    ghost_assn\<^sup>k *\<^sub>a (list_assn (list_assn unat_lit_assn))\<^sup>d *\<^sub>a
      (isasat_input_ops.isasat_init_fast_assn \<A>\<^sub>i\<^sub>n)\<^sup>d \<rightarrow>
     isasat_input_ops.isasat_init_fast_assn \<A>\<^sub>i\<^sub>n\<close>
   unfolding PR_CONST_def
@@ -220,7 +200,7 @@ lemma init_dt_wl_fast_code_refine[sepref_fr_rules]:
       rule_format, of \<open>(snd (fst c), snd c)\<close> \<open>(snd (fst a), snd a)\<close>]
     by (cases a)
        (sep_auto dest!: frame_rule_left[of \<open>_ * isasat_input_ops.isasat_init_fast_assn _ _ _\<close> _ _
-            \<open>virtual_copy_assn \<A>\<^sub>i\<^sub>n (fst (fst a))\<close>])
+            \<open>ghost_assn \<A>\<^sub>i\<^sub>n (fst (fst a))\<close>])
   done *)
 
 definition (in -)convert_state where
@@ -229,7 +209,7 @@ definition (in -)convert_state where
 lemma (in -) convert_state_hnr:
   \<open>(uncurry (return oo (\<lambda>_ S. S)), uncurry (RETURN oo convert_state))
    \<in> [\<lambda>(N, S). N = \<A>\<^sub>i\<^sub>n \<and> N = \<A>\<^sub>i\<^sub>n']\<^sub>a
-     virtual_copy_assn\<^sup>k *\<^sub>a (isasat_input_ops.isasat_init_assn \<A>\<^sub>i\<^sub>n)\<^sup>d \<rightarrow>
+     ghost_assn\<^sup>k *\<^sub>a (isasat_input_ops.isasat_init_assn \<A>\<^sub>i\<^sub>n)\<^sup>d \<rightarrow>
      isasat_input_ops.isasat_init_assn \<A>\<^sub>i\<^sub>n'\<close>
   by sepref_to_hoare (sep_auto simp: convert_state_def)
 (*
@@ -237,7 +217,7 @@ lemma (in -) convert_state_hnr:
 lemma (in -) convert_state_fast_hnr:
   \<open>(uncurry (return oo (\<lambda>_ S. S)), uncurry (RETURN oo convert_state))
    \<in> [\<lambda>(N, S). N = \<A>\<^sub>i\<^sub>n \<and> N = \<A>\<^sub>i\<^sub>n']\<^sub>a
-     virtual_copy_assn\<^sup>k *\<^sub>a (isasat_input_ops.isasat_init_fast_assn \<A>\<^sub>i\<^sub>n)\<^sup>d \<rightarrow>
+     ghost_assn\<^sup>k *\<^sub>a (isasat_input_ops.isasat_init_fast_assn \<A>\<^sub>i\<^sub>n)\<^sup>d \<rightarrow>
      isasat_input_ops.isasat_init_fast_assn \<A>\<^sub>i\<^sub>n'\<close>
   by sepref_to_hoare (sep_auto simp: convert_state_def) *)
 
@@ -311,7 +291,7 @@ lemma in_class_in_literals_are_in_\<L>\<^sub>i\<^sub>n:
   apply (subst insert_absorb[OF assms, symmetric])
   apply auto
   done
-
+(* TODO Move *)
 lemma (in -)id_mset_list_assn_list_mset_assn:
   assumes \<open>CONSTRAINT is_pure R\<close>
   shows \<open>(return o id, RETURN o mset) \<in> (list_assn R)\<^sup>d \<rightarrow>\<^sub>a list_mset_assn R\<close>
@@ -327,11 +307,11 @@ proof -
     by (sep_auto simp: list_mset_assn_def R' pure_def list_mset_rel_def mset_rel_def
        p2rel_def rel2p_def[abs_def] rel_mset_def br_def Collect_eq_comp list_rel_def)
 qed
-
+(* END Move *)
 lemma cdcl_twl_stgy_prog_wl_D_code_ref':
   \<open>(uncurry (\<lambda>_. cdcl_twl_stgy_prog_wl_D_code), uncurry isasat_input_ops.cdcl_twl_stgy_prog_wl_D_heur)
   \<in> [\<lambda>(N, _). N = \<A>\<^sub>i\<^sub>n \<and> isasat_input_bounded_nempty \<A>\<^sub>i\<^sub>n]\<^sub>a
-     (virtual_copy_assn)\<^sup>k *\<^sub>a
+     (ghost_assn)\<^sup>k *\<^sub>a
     (isasat_input_ops.isasat_assn \<A>\<^sub>i\<^sub>n)\<^sup>d \<rightarrow> isasat_input_ops.isasat_assn \<A>\<^sub>i\<^sub>n\<close>
   unfolding hfref_def hn_refine_def
   apply (subst in_pair_collect_simp)
@@ -343,7 +323,7 @@ lemma cdcl_twl_stgy_prog_wl_D_code_ref':
     apply (cases a)
     by (sep_auto simp:
       dest!: frame_rule_left[of \<open>isasat_input_ops.isasat_assn _ _ _\<close> _ _
-        \<open>virtual_copy_assn \<A>\<^sub>i\<^sub>n (fst a)\<close>])
+        \<open>ghost_assn \<A>\<^sub>i\<^sub>n (fst a)\<close>])
   done
 
 (*
@@ -351,7 +331,7 @@ lemma cdcl_twl_stgy_prog_wl_D_break_fast_code_ref':
   \<open>(uncurry (\<lambda>_. cdcl_twl_stgy_prog_wl_D_fast_code),
       uncurry isasat_input_ops.cdcl_twl_stgy_prog_break_wl_D_heur_break)
   \<in> [\<lambda>(N, S). N = \<A>\<^sub>i\<^sub>n \<and> isasat_input_bounded_nempty \<A>\<^sub>i\<^sub>n \<and> isasat_fast S]\<^sub>a
-     (virtual_copy_assn)\<^sup>k *\<^sub>a
+     (ghost_assn)\<^sup>k *\<^sub>a
     (isasat_input_ops.isasat_fast_assn \<A>\<^sub>i\<^sub>n)\<^sup>d \<rightarrow> isasat_input_ops.isasat_assn \<A>\<^sub>i\<^sub>n\<close>
   unfolding hfref_def hn_refine_def
   apply (subst in_pair_collect_simp)
@@ -363,7 +343,7 @@ lemma cdcl_twl_stgy_prog_wl_D_break_fast_code_ref':
     by (cases a)
       (sep_auto simp:
       dest!: frame_rule_left[of \<open>isasat_input_ops.isasat_fast_assn _ _ _\<close> _ _
-       \<open>virtual_copy_assn \<A>\<^sub>i\<^sub>n (fst a)\<close>])
+       \<open>ghost_assn \<A>\<^sub>i\<^sub>n (fst a)\<close>])
   done *)
 
 declare cdcl_twl_stgy_prog_wl_D_code_ref'[to_hnr, OF refl, sepref_fr_rules]
