Weidenbach_Book/IsaSAT_Arena.thy
@@ -4,31 +4,6 @@ imports IsaSAT_Literals
   Watched_Literals.WB_Word_Assn
 begin
 
-(* TODO Move + add 64 bits version *)
-lemma bitAND_uint32_nat_assn[sepref_fr_rules]:
-  \<open>(uncurry (return oo (AND)), uncurry (RETURN oo (AND))) \<in> 
-    uint32_nat_assn\<^sup>k *\<^sub>a uint32_nat_assn\<^sup>k \<rightarrow>\<^sub>a uint32_nat_assn\<close>
-  by sepref_to_hoare
-    (sep_auto simp: uint32_nat_rel_def br_def nat_of_uint32_ao)
-
-lemma bitAND_uint32_assn[sepref_fr_rules]:
-  \<open>(uncurry (return oo (AND)), uncurry (RETURN oo (AND))) \<in> 
-    uint32_assn\<^sup>k *\<^sub>a uint32_assn\<^sup>k \<rightarrow>\<^sub>a uint32_assn\<close>
-  by sepref_to_hoare
-    (sep_auto simp: uint32_nat_rel_def br_def nat_of_uint32_ao)
-
-lemma bitOR_uint32_nat_assn[sepref_fr_rules]:
-  \<open>(uncurry (return oo (OR)), uncurry (RETURN oo (OR))) \<in> 
-    uint32_nat_assn\<^sup>k *\<^sub>a uint32_nat_assn\<^sup>k \<rightarrow>\<^sub>a uint32_nat_assn\<close>
-  by sepref_to_hoare
-    (sep_auto simp: uint32_nat_rel_def br_def nat_of_uint32_ao)
-
-lemma bitOR_uint32_assn[sepref_fr_rules]:
-  \<open>(uncurry (return oo (OR)), uncurry (RETURN oo (OR))) \<in> 
-    uint32_assn\<^sup>k *\<^sub>a uint32_assn\<^sup>k \<rightarrow>\<^sub>a uint32_assn\<close>
-  by sepref_to_hoare
-    (sep_auto simp: uint32_nat_rel_def br_def nat_of_uint32_ao)
-(* END Move *)
 
 subsection \<open>The memory representation: Arenas\<close>
 
